Fixed cheats for disjunction theorem in case of unknown table configuration

hol/symb_exec/p4_symb_execScript.sml
@@ -186,6 +186,7 @@ rpt strip_tac >> (
 )
 QED
 
+(* TODO: Annoying that entire ascope is used. You can make more efficient versions that only use ctrl, tailored for individual architectures. *)
 Definition ctrl_is_well_formed_def:
  ctrl_is_well_formed (ftymap, blftymap, pblock_action_names_map) (pblock_map:pblock_map, apply_table_f:'a apply_table_f) (ascope:'a) =
   !block_name pbl_type x_d_list b_func_map decl_list pars_map tbl_map action_names_map.
@@ -194,19 +195,34 @@ Definition ctrl_is_well_formed_def:
     !tbl mk_l actions default_f default_f_args.
      ALOOKUP tbl_map tbl = SOME (mk_l, (default_f, default_f_args)) ==>
      ALOOKUP action_names_map tbl = SOME actions ==>
-      !e_l. ?f f_args.
+      !e_l.
+      (* TODO: Keep the requirement that LENGTH e_l = LENGTH mk_l here? *)
+      LENGTH e_l = LENGTH mk_l ==>
+      ?f f_args.
       apply_table_f (tbl, e_l, mk_l, (default_f, default_f_args), ascope) = SOME (f, f_args) /\
+       (* f is in the list of actions for the table *)
        MEM f actions /\
-       (EL 0 f_args = (e_v (v_bool T))) /\
-       (f = default_f ==> ?b. EL 1 f_args = (e_v (v_bool b))) /\
-       (f <> default_f ==> EL 1 f_args = (e_v (v_bool T))) /\
-       ((?ftys ret_ty local_ftymap. ALOOKUP blftymap block_name = SOME local_ftymap /\
-        ALOOKUP local_ftymap (funn_name f) = SOME (ftys, ret_ty:tau) /\
-        v_to_tau_list (DROP 2 f_args) = SOME (ftys)) \/
-       (ALOOKUP blftymap block_name = NONE \/
-        (?local_ftymap.
+       (* first argument is the Boolean T, signifying that the function call resulted from table application *)
+       (oEL 0 f_args = SOME (e_v (v_bool T))) /\
+       (* first argument is either:
+        * a Boolean, if action name is that of the default action... *)
+       (f = default_f ==> ?b. oEL 1 f_args = SOME (e_v (v_bool b))) /\
+       (* or the Boolean T, if action name is not that of the default action. *)
+       (f <> default_f ==> oEL 1 f_args = SOME (e_v (v_bool T))) /\
+       (* Furthermore, the types of the arguments must agree with those associated with the action
+        * in the relevant ftymap. *)
+       (* Case 1: Block name is found in blftymap, and function name in the local ftymap.
+         * Then, that local function type map applies. *)
+       ((?ftys ret_ty local_ftymap.
          ALOOKUP blftymap block_name = SOME local_ftymap /\
-         ALOOKUP local_ftymap (funn_name f) = NONE) /\
+         ALOOKUP local_ftymap (funn_name f) = SOME (ftys, ret_ty:tau) /\
+         v_to_tau_list (DROP 2 f_args) = SOME (ftys)) \/
+        (* Case 2: Either block name can't be found in blftymap, or function name can't be found in local ftymap.
+         * Then, the global function type map applies. *)
+        (ALOOKUP blftymap block_name = NONE \/
+         (?local_ftymap.
+          ALOOKUP blftymap block_name = SOME local_ftymap /\
+          ALOOKUP local_ftymap (funn_name f) = NONE) /\
         (?ftys ret_ty. ALOOKUP ftymap (funn_name f) = SOME (ftys, ret_ty:tau) /\
          v_to_tau_list (DROP 2 f_args) = SOME (ftys))))
 End
